updates
Signed-off-by: Shaobo He <shaobohe@amazon.com>

cedar-lean/Cedar/TPE/Input.lean
@@ -50,7 +50,7 @@ structure PartialEntityData where
 
 abbrev PartialEntities := Map EntityUID PartialEntityData
 
-private def PartialEntities.get (es : PartialEntities) (uid : EntityUID) (f : PartialEntityData → Option α) : Option α :=
+def PartialEntities.get (es : PartialEntities) (uid : EntityUID) (f : PartialEntityData → Option α) : Option α :=
   (es.find? uid).bind f
 
 def PartialEntities.ancestors (es : PartialEntities) (uid : EntityUID) : Option (Set EntityUID) := es.get uid PartialEntityData.ancestors
